saving work - proof of new RealSimp step

uc-dsl/examples/smc2/DDH.ec
@@ -1,73 +1,553 @@
-(* DDH.ec *)
+(* DDH.h *)
 
-(* Decisional Diffie-Hellman Assumption *)
+(* Decisional Diffie-Hellman Assumptions, Eager and Lazy *)
 
-prover [""].  (* no provers *)
-
-require import AllCore Distr.
+require import AllCore Distr FMap PROM.
 
 (*************************** Begin Theory Parameters **************************)
 
-(* group of keys *)
+type input.  (* additional input to adversary *)
 
-type key.
+type key.  (* keys *)
 
-op (^^) : key -> key -> key.  (* binary operation *)
-
-(* commutative semigroup of exponents *)
-
-type exp.
+type exp.  (* exponents *)
 
 op ( * ) : exp -> exp -> exp.  (* multiplication *)
 
-(* full (every element has non-zero weight), uniform (all elements
-   with non-zero weight have same weight) and lossless (sum of all
-   weights is 1%r) distribution over exp
-
-   consequently exp has only finitely many elements *)
-
 op [full uniform lossless] dexp : exp distr.
-
-(* connection between key and exp, via generator key and
-   exponentiation operation *)
 
 op g : key.  (* generator *)
 
 op (^) : key -> exp -> key.  (* exponentiation *)
 
+(* more axioms will hold, but this is all we need in this theory *)
+
 (**************************** End Theory Parameters ***************************)
 
 (******************** Decisional Diffie-Hellman Assumption ********************)
 
+(* this is the normal, "eager", DDH assumption, in which the
+   exponents are chosen at the beginning of the games
+
+   the two games take in a value of type input, which is passed
+   to the adversary *)
+
 (* DDH Adversary *)
 
 module type DDH_ADV = {
-  proc main(k1 k2 k3 : key) : bool
+  proc main(x : input, k1 k2 k3 : key) : bool
 }.
 
 module DDH1 (Adv : DDH_ADV) = {
-  proc main() : bool = {
+  proc main(x : input) : bool = {
     var b : bool; var q1, q2 : exp;
     q1 <$ dexp; q2 <$ dexp;
-    b <@ Adv.main(g ^ q1, g ^ q2, g ^ (q1 * q2));
+    b <@ Adv.main(x, g ^ q1, g ^ q2, g ^ (q1 * q2));
     return b;
   }
 }.
   
 module DDH2 (Adv : DDH_ADV) = {
-  proc main() : bool = {
+  proc main(x : input) : bool = {
     var b : bool; var q1, q2, q3 : exp;
     q1 <$ dexp; q2 <$ dexp; q3 <$ dexp;
-    b <@ Adv.main(g ^ q1, g ^ q2 , g ^ q3);
+    b <@ Adv.main(x, g ^ q1, g ^ q2 , g ^ q3);
     return b;
   }
 }.
 
-(* the *advantage* of a DDH adversary Adv is
+(* for all x : input, the *advantage* of a DDH adversary Adv is
 
-   `|Pr[DDH1(Adv).main() @ &m : res] - Pr[DDH2(Adv).main() @ &m : res]|
+   `|Pr[DDH1(Adv).main(x) @ &m : res] - Pr[DDH2(Adv).main(x) @ &m : res]|
 
-   this will be negligible under certain assumptions about the group
-   key, the commutative semigroup exp, and the efficiency of Adv
-   (including that Adv doesn't compute the inverse of fun q => g ^
-   q *)
+   this will be negligible under certain assumptions about key, exp
+   and the efficiency of Adv (including that Adv doesn't compute the
+   inverse of fun q => g ^ q) *)
+
+(***************** Lazy Decisional Diffie-Hellman Assumption ****************)
+
+(* a "lazy", oracle-based version of the Decisional Diffie-Hellman
+   assumption, with two oracles (DDH_Or1 and DDH_Or2) and a single
+   game using them
+
+   the exponents are only generated (and cached) by the oracles when
+   keys are requested by the adversary
+
+   the third key may only be requested (otherwise witness is returned)
+   after the first two have been (in either order) *)
+
+type three = [One | Two | Three].
+
+module type DDH_OR = {
+  proc init() : unit         (* initialization *)
+  proc get(i : three) : key  (* get on of the three keys *)
+}.
+
+module DDH1_Or : DDH_OR = {
+  var x_opt : exp option
+  var y_opt : exp option
+
+  proc init() : unit = {
+    x_opt <- None; y_opt <- None;
+  }
+
+  proc get(i : three) : key = {
+    var r : key; var x, y : exp;
+    match i with
+    | One   => {
+        if (x_opt = None) {
+          x <$ dexp; x_opt <- Some x;
+        }
+        r <- g ^ oget x_opt;
+      }
+    | Two   => {
+        if (y_opt = None) {
+          y <$ dexp; y_opt <- Some y;
+        }
+        r <- g ^ oget y_opt;
+      }
+    | Three => {
+        (* witness is returned unless both of x and y have
+           already been generated *)
+        if (x_opt <> None /\ y_opt <> None) {
+          r <- g ^ (oget x_opt * oget y_opt);
+        }
+        else { r <- witness; }
+      }
+    end;
+    return r;
+  }
+}.
+
+module DDH2_Or : DDH_OR = {
+  var x_opt : exp option
+  var y_opt : exp option
+  var z_opt : exp option
+
+  proc init() : unit = {
+    x_opt <- None; y_opt <- None; z_opt <- None;
+  }
+
+  proc get(i : three) : key = {
+    var r : key; var x, y, z : exp;
+    match i with
+    | One   => {
+        if (x_opt = None) {
+          x <$ dexp; x_opt <- Some x;
+        }
+        r <- g ^ oget x_opt;
+      }
+    | Two   => {
+        if (y_opt = None) {
+          y <$ dexp; y_opt <- Some y;
+        }
+        r <- g ^ oget y_opt;
+      }
+    | Three => {
+        (* witness is returned unless both x and y have
+           already been generated *)
+        if (x_opt <> None /\ y_opt <> None) {
+          if (z_opt = None) {
+            z <$ dexp; z_opt <- Some z;
+          }
+          r <- g ^ oget z_opt;
+        }
+        else { r <- witness; }
+      }
+    end;
+    return r;
+  }
+}.
+
+(* module type of DDH oracle adversaries
+
+   the adversary cannot reinitialize the oracle *)
+
+module type DDH_OR_ADV (Or : DDH_OR) = {
+  proc main(x : input) : bool {Or.get}
+}.
+
+module DDH_Or_Game (Or : DDH_OR, Adv : DDH_OR_ADV) = {
+  proc main(x : input) : bool = {
+    var b : bool;
+    Or.init();
+    b <@ Adv(Or).main(x);
+    return b;
+  }
+}.
+
+(* convert a DDH oracle adversary to an ordinary DDH
+   adversary *)
+
+module DDH_Adv_Conv (Adv : DDH_OR_ADV) : DDH_ADV = {
+  module Or : DDH_OR = {
+    var k1, k2, k3 : key
+    var one, two : bool  (* have the first two keys been requested? *)
+
+    proc init() : unit = { }
+
+    proc get(i : three) : key = {
+      var r : key;
+      match i with
+      | One   => { r <- k1; one <- true; }
+      | Two   => { r <- k2; two <- true; }
+      | Three => {
+          (* witness is returned if the first two keys have
+             not already been requested *)
+          if (one /\ two) { r <- k3; }
+          else { r <- witness; }
+        }
+      end;
+      return r;
+    }
+  }
+
+  proc main(x : input, k1 : key, k2 : key, k3 : key) : bool = {
+    var b : bool;
+    Or.k1 <- k1; Or.k2 <- k2; Or.k3 <- k3;
+    Or.one <- false; Or.two <- false;
+    b <@ Adv(Or).main(x);
+    return b;
+  }
+}.
+
+(* skip to the end of the section to see the first main lemma *)
+        
+section.
+
+declare module Adv <: DDH_OR_ADV{-DDH_Adv_Conv, -DDH1_Or}.
+
+(* we use eager/lazy sampling - see PROM *)
+
+local clone FullRO with
+  type in_t    <- three,
+  type out_t   <- exp,
+  op dout      <- fun _ => dexp,
+  type d_in_t  <- input,
+  type d_out_t <- bool
+proof *.
+
+local module (RO_Disting1 : FullRO.RO_Distinguisher) (RO : FullRO.RO) = {
+  module Or : DDH_OR = {
+    var one, two : bool
+
+    proc init() : unit = { }
+
+    proc get(i : three) : key = {
+      var r : key; var x, y : exp;
+      match i with
+      | One   => {
+          x <@ RO.get(One); one <- true;
+          r <- g ^ x;
+        }
+      | Two   => {
+          y <@ RO.get(Two); two <- true;
+          r <- g ^ y;
+        }
+      | Three => {
+          if (one /\ two) {
+            x <@ RO.get(One);
+            y <@ RO.get(Two);
+            r <- g ^ (x * y);
+          }
+          else { r <- witness; }
+        }
+      end;
+      return r;
+    }
+  }
+
+  proc distinguish(x : input) : bool = {
+    var b : bool;
+    Or.one <- false; Or.two <- false;
+    (* sample either eagerly or lazily *)
+    RO.sample(One); RO.sample(Two);
+    b <@ Adv(Or).main(x);
+    return b;
+  }
+}.
+
+local lemma first (x' : input) &m :
+  Pr[DDH_Or_Game(DDH1_Or, Adv).main(x') @ &m : res] =
+  Pr[FullRO.MainD(RO_Disting1, FullRO.LRO).distinguish(x') @ &m : res].
+proof.
+byequiv (_ : ={x, glob Adv} ==> _) => //; proc; inline*; wp.
+seq 2 6 :
+  (={glob Adv} /\ x{1} = x0{2} /\
+   DDH1_Or.x_opt{1} = FullRO.RO.m{2}.[One] /\
+   DDH1_Or.y_opt{1} = FullRO.RO.m{2}.[Two] /\
+   (DDH1_Or.x_opt{1} = None <=> ! RO_Disting1.Or.one{2}) /\
+   (DDH1_Or.y_opt{1} = None <=> ! RO_Disting1.Or.two{2})).
+auto; smt(emptyE).
+call
+  (_ : 
+   DDH1_Or.x_opt{1} = FullRO.RO.m{2}.[One] /\
+   DDH1_Or.y_opt{1} = FullRO.RO.m{2}.[Two] /\
+   (DDH1_Or.x_opt{1} = None <=> ! RO_Disting1.Or.one{2}) /\
+   (DDH1_Or.y_opt{1} = None <=> ! RO_Disting1.Or.two{2})).
+proc; match => //.
+inline{2} 1.
+case (DDH1_Or.x_opt{1} = None).
+rcondt{1} 1; first auto.
+rcondt{2} 3; first auto.
+swap{2} 2 -1; wp; rnd; auto; smt(get_setE).
+rcondf{1} 1; first auto.
+rcondf{2} 3; first auto.
+swap{2} 2 -1; wp; rnd{2}; auto.
+inline{2} 1.
+case (DDH1_Or.y_opt{1} = None).
+rcondt{1} 1; first auto.
+rcondt{2} 3; first auto.
+swap{2} 2 -1; wp; rnd; auto; smt(get_setE).
+rcondf{1} 1; first auto.
+rcondf{2} 3; first auto.
+swap{2} 2 -1; wp; rnd{2}; auto.
+inline*.
+if; first smt().
+rcondf{2} 3; first auto.
+rcondf{2} 6; first auto.
+auto.
+auto.
+auto.
+qed.
+
+local lemma second (x : input) &m :
+  Pr[FullRO.MainD(RO_Disting1, FullRO.LRO).distinguish(x) @ &m : res] =
+  Pr[FullRO.MainD(RO_Disting1, FullRO.RO).distinguish(x) @ &m : res].
+proof.
+byequiv
+  (_ :
+   ={x, glob Adv, RO_Disting1.Or.one, RO_Disting1.Or.two} ==> _) => //.
+symmetry.
+conseq (FullRO.FullEager.RO_LRO RO_Disting1 _) => //.
+smt(dexp_ll).
+qed.
+
+local lemma third (x : input) &m :
+  Pr[FullRO.MainD(RO_Disting1, FullRO.RO).distinguish(x) @ &m : res] =
+  Pr[DDH1(DDH_Adv_Conv(Adv)).main(x) @ &m : res].
+proof.
+byequiv (_ : ={x, glob Adv} ==> _) => //; proc; inline*; wp.
+rcondt{1} 8; first auto; smt(emptyE).
+rcondt{1} 12; first auto; smt(mem_set mem_empty).
+swap{1} 7 -6; swap{1} 11 -9.
+seq 12 11 :
+  (={x0, glob Adv} /\ ={one, two}(RO_Disting1.Or, DDH_Adv_Conv.Or) /\
+   FullRO.RO.m{1} = (empty.[One <- r0{1}]).[Two <- r1{1}] /\
+   DDH_Adv_Conv.Or.k1{2} = g ^ r0{1} /\ DDH_Adv_Conv.Or.k2{2} = g ^ r1{1} /\
+   DDH_Adv_Conv.Or.k3{2} = g ^ (r0{1} * r1{1})).
+wp; rnd; rnd; auto.
+exlim r0{1}, r1{1} => r0_L r1_L.
+call
+  (_ :
+   ={one, two}(RO_Disting1.Or, DDH_Adv_Conv.Or) /\
+   FullRO.RO.m{1} = (empty.[One <- r0_L]).[Two <- r1_L] /\
+   DDH_Adv_Conv.Or.k1{2} = g ^ r0_L /\ DDH_Adv_Conv.Or.k2{2} = g ^ r1_L /\
+   DDH_Adv_Conv.Or.k3{2} = g ^ (r0_L * r1_L)).
+proc.
+match => //.
+inline*.
+rcondf{1} 3; first auto; smt(mem_set).
+auto; smt(get_setE).
+inline*.
+rcondf{1} 3; first auto; smt(mem_set).
+auto; smt(get_setE).
+if => //.
+inline*.
+rcondf{1} 3; first auto; smt(mem_set).
+rcondf{1} 6; first auto; smt(mem_set).
+auto; smt(get_setE).
+auto.
+auto.
+qed.
+
+lemma Reduction1' (x : input) &m :
+  Pr[DDH_Or_Game(DDH1_Or, Adv).main(x) @ &m : res] =
+  Pr[DDH1(DDH_Adv_Conv(Adv)).main(x) @ &m : res].
+proof. by rewrite first second third. qed.
+
+end section.
+
+lemma Reduction1 (Adv <: DDH_OR_ADV{-DDH_Adv_Conv, -DDH1_Or}) (x : input) &m :
+  Pr[DDH_Or_Game(DDH1_Or, Adv).main(x) @ &m : res] =
+  Pr[DDH1(DDH_Adv_Conv(Adv)).main(x) @ &m : res].
+proof. by rewrite (Reduction1' Adv). qed.
+
+(* skip to the end of the section to see the second main lemma *)
+
+section.
+
+declare module Adv <: DDH_OR_ADV{-DDH_Adv_Conv, -DDH2_Or}.
+
+local clone FullRO with
+  type in_t    <- three,
+  type out_t   <- exp,
+  op dout      <- fun _ => dexp,
+  type d_in_t  <- input,
+  type d_out_t <- bool
+proof *.
+
+local module (RO_Disting2 : FullRO.RO_Distinguisher) (RO : FullRO.RO) = {
+  module Or : DDH_OR = {
+    var one, two : bool
+
+    proc init() : unit = { }
+
+    proc get(i : three) : key = {
+      var r : key; var x, y, z : exp;
+      match i with
+      | One   => {
+          x <@ RO.get(One); one <- true;
+          r <- g ^ x;
+        }
+      | Two   => {
+          y <@ RO.get(Two); two <- true;
+          r <- g ^ y;
+        }
+      | Three => {
+          if (one /\ two) {
+            z <@ RO.get(Three);
+            r <- g ^ z;
+          }
+          else { r <- witness; }
+        }
+      end;
+      return r;
+    }
+  }
+
+  proc distinguish(x : input) : bool = {
+    var b : bool;
+    Or.one <- false; Or.two <- false;
+    (* sample either eagerly or lazily *)
+    RO.sample(One); RO.sample(Two); RO.sample(Three);
+    b <@ Adv(Or).main(x);
+    return b;
+  }
+}.
+
+local lemma first (x' : input) &m :
+  Pr[DDH_Or_Game(DDH2_Or, Adv).main(x') @ &m : res] =
+  Pr[FullRO.MainD(RO_Disting2, FullRO.LRO).distinguish(x') @ &m : res].
+proof.
+byequiv (_ : ={x, glob Adv} ==> _) => //; proc; inline*; wp.
+seq 3 7 :
+  (={glob Adv} /\ x{1} = x0{2} /\
+   DDH2_Or.x_opt{1} = FullRO.RO.m{2}.[One] /\
+   DDH2_Or.y_opt{1} = FullRO.RO.m{2}.[Two] /\
+   DDH2_Or.z_opt{1} = FullRO.RO.m{2}.[Three] /\
+   (DDH2_Or.x_opt{1} = None <=> ! RO_Disting2.Or.one{2}) /\
+   (DDH2_Or.y_opt{1} = None <=> ! RO_Disting2.Or.two{2})).
+auto; smt(emptyE).
+call
+  (_ : 
+   DDH2_Or.x_opt{1} = FullRO.RO.m{2}.[One] /\
+   DDH2_Or.y_opt{1} = FullRO.RO.m{2}.[Two] /\
+   DDH2_Or.z_opt{1} = FullRO.RO.m{2}.[Three] /\
+   (DDH2_Or.x_opt{1} = None <=> ! RO_Disting2.Or.one{2}) /\
+   (DDH2_Or.y_opt{1} = None <=> ! RO_Disting2.Or.two{2})).
+proc; match => //.
+inline{2} 1.
+case (DDH2_Or.x_opt{1} = None).
+rcondt{1} 1; first auto.
+rcondt{2} 3; first auto.
+swap{2} 2 -1; wp; rnd; auto; smt(get_setE).
+rcondf{1} 1; first auto.
+rcondf{2} 3; first auto.
+swap{2} 2 -1; wp; rnd{2}; auto.
+inline{2} 1.
+case (DDH2_Or.y_opt{1} = None).
+rcondt{1} 1; first auto.
+rcondt{2} 3; first auto.
+swap{2} 2 -1; wp; rnd; auto; smt(get_setE).
+rcondf{1} 1; first auto.
+rcondf{2} 3; first auto.
+swap{2} 2 -1; wp; rnd{2}; auto.
+inline*.
+if; first smt().
+case (DDH2_Or.z_opt{1} = None).
+rcondt{1} 1; first auto.
+rcondt{2} 3; first auto.
+swap{2} 2 -1; wp; rnd.
+auto; progress; by rewrite get_setE.
+rcondf{1} 1; first auto.
+rcondf{2} 3; first auto.
+auto.
+auto.
+auto.
+qed.
+
+local lemma second (x : input) &m :
+  Pr[FullRO.MainD(RO_Disting2, FullRO.LRO).distinguish(x) @ &m : res] =
+  Pr[FullRO.MainD(RO_Disting2, FullRO.RO).distinguish(x) @ &m : res].
+proof.
+byequiv
+  (_ :
+   ={x, glob Adv, RO_Disting2.Or.one, RO_Disting2.Or.two} ==> _) => //.
+symmetry.
+conseq (FullRO.FullEager.RO_LRO RO_Disting2 _) => //.
+smt(dexp_ll).
+qed.
+
+local lemma third (x : input) &m :
+  Pr[FullRO.MainD(RO_Disting2, FullRO.RO).distinguish(x) @ &m : res] =
+  Pr[DDH2(DDH_Adv_Conv(Adv)).main(x) @ &m : res].
+proof.
+byequiv (_ : ={x, glob Adv} ==> _) => //; proc; inline*; wp.
+rcondt{1} 8; first auto; smt(emptyE).
+rcondt{1} 12; first auto; smt(mem_set mem_empty).
+rcondt{1} 16; first auto; smt(mem_set mem_empty).
+swap{1} 7 -6; swap{1} 11 -9; swap{1} 15 -12.
+seq 16 12 :
+  (={x0, glob Adv} /\ ={one, two}(RO_Disting2.Or, DDH_Adv_Conv.Or) /\
+   FullRO.RO.m{1} =
+   ((empty.[One <- r0{1}]).[Two <- r1{1}]).[Three <- r2{1}] /\
+   DDH_Adv_Conv.Or.k1{2} = g ^ r0{1} /\ DDH_Adv_Conv.Or.k2{2} = g ^ r1{1} /\
+   DDH_Adv_Conv.Or.k3{2} = g ^ r2{1}).
+wp; rnd; rnd; rnd; auto.
+exlim r0{1}, r1{1}, r2{1} => r0_L r1_L r2_L.
+call
+  (_ :
+   ={one, two}(RO_Disting2.Or, DDH_Adv_Conv.Or) /\
+   FullRO.RO.m{1} =
+   ((empty.[One <- r0_L]).[Two <- r1_L]).[Three <- r2_L] /\
+   DDH_Adv_Conv.Or.k1{2} = g ^ r0_L /\ DDH_Adv_Conv.Or.k2{2} = g ^ r1_L /\
+   DDH_Adv_Conv.Or.k3{2} = g ^ r2_L).
+proc; match => //.
+inline*.
+rcondf{1} 3; first auto; smt(mem_set).
+auto; smt(get_setE).
+inline*.
+rcondf{1} 3; first auto; smt(mem_set).
+auto; smt(get_setE).
+if => //.
+inline*.
+rcondf{1} 3; first auto; smt(mem_set).
+auto; smt(get_setE).
+auto.
+auto.
+qed.
+
+lemma Reduction2' (x : input) &m :
+  Pr[DDH_Or_Game(DDH2_Or, Adv).main(x) @ &m : res] =
+  Pr[DDH2(DDH_Adv_Conv(Adv)).main(x) @ &m : res].
+proof. by rewrite first second third. qed.
+
+end section.
+
+lemma Reduction2 (Adv <: DDH_OR_ADV{-DDH_Adv_Conv, -DDH2_Or})
+                 (x : input) &m :
+  Pr[DDH_Or_Game(DDH2_Or, Adv).main(x) @ &m : res] =
+  Pr[DDH2(DDH_Adv_Conv(Adv)).main(x) @ &m : res].
+proof. by rewrite (Reduction2' Adv). qed.
+
+(* our main result, reducing lazy decisional Diffie-Hellman
+   to ordinary (eager) decisional Diffie-Hellman *)
+
+lemma Reduction (Adv <: DDH_OR_ADV{-DDH_Adv_Conv, -DDH1_Or, -DDH2_Or})
+                (x : input) &m :
+  `|Pr[DDH_Or_Game(DDH1_Or, Adv).main(x) @ &m : res] -
+    Pr[DDH_Or_Game(DDH2_Or, Adv).main(x) @ &m : res]| =
+  `|Pr[DDH1(DDH_Adv_Conv(Adv)).main(x) @ &m : res] -
+    Pr[DDH2(DDH_Adv_Conv(Adv)).main(x) @ &m : res]|.
+proof. by rewrite (Reduction1 Adv) (Reduction2 Adv). qed.
